\begin{answer}

\begin{equation*}
p(t^{(i)}=1\mid y^{(i)} = 1, x^{(i)}) = \frac{p(y^{(i)}=1\mid t^{(i)} = 1, x^{(i)})p(t^{(i)}=1\mid x^{(i)})}{p(y^{(i)}=1\mid t^{(i)} = 1, x^{(i)})p(t^{(i)}=1\mid x^{(i)}) + p(y^{(i)}=1\mid t^{(i)} = 0, x^{(i)})p(t^{(i)}=0\mid x^{(i)})} = 
\end{equation*}

\begin{equation*}
\frac{1}{1 + \frac{p(y^{(i)}=1\mid t^{(i)} = 0, x^{(i)})p(t^{(i)}=0\mid x^{(i)})}{p(y^{(i)}=1\mid t^{(i)} = 1, x^{(i)})p(t^{(i)}=1\mid x^{(i)}) }} = \frac{1}{1 + 0} = 1
\end{equation*}

\end{answer}
