\begin{answer}

\begin{equation*}
	p(y=1|x; \phi, \mu_0, \mu_1, \Sigma) =  \frac{p(x|y=1)p(y=1)}{p(x|y=1)p(y=1) + p(x|y=0)p(y=0)} = 
\end{equation*}

\begin{equation*}
	\frac{1}{1 + \frac{p(x|y=0)p(y=0)}{p(x|y=1)p(y=1)}} = \frac{1}{1 + \frac{1-\phi}{\phi} \exp(-1/2( (x-\mu_{0})^T \Sigma^{-1} (x-\mu_{0}) - (x-\mu_{1})^T \Sigma^{-1} (x-\mu_{1}) ))} = 
\end{equation*}

\begin{equation*}
\frac{1}{1 + \exp(-(\frac{1}{2}( \mu_{0}^T \Sigma^{-1} \mu_{0} - \mu_{1}^T \Sigma^{-1} \mu_{1} ) + \log(\frac{\phi}{1 - \phi}) + (\mu_1^T\Sigma^{-1} - \mu_0^T\Sigma^{-1})x))}
\end{equation*}

\end{answer}
