<<<<<<< HEAD
\begin{answer}
$$\ell_\text{semi-sup}(\theta^{(t+1)}) \ge \sum_{i=1}^{\nexp} ELBO(x^{(i)}; Q^{(t)}, \theta^{(t+1)}) + \alpha \sum_{i=1}^{\nexp} LL(\tilde{x}^{(i)}, \tilde{z}^{(i)}; \theta^{(t+1)}))  \ge$$
$$\sum_{i=1}^{\nexp} ELBO(x^{(i)}; Q^{(t)}, \theta^{(t)}) + \alpha \sum_{i=1}^{\nexp} LL(\tilde{x}^{(i)}, \tilde{z}^{(i)}; \theta^{(t)}) = \ell_\text{semi-sup}(\theta^{(t)})$$
\end{answer}
=======
\begin{answer}
$$\ell_\text{semi-sup}(\theta^{(t+1)}) \ge \sum_{i=1}^{\nexp} ELBO(x^{(i)}; Q^{(t)}, \theta^{(t+1)}) + \alpha \sum_{i=1}^{\nexp} LL(\tilde{x}^{(i)}, \tilde{z}^{(i)}; \theta^{(t+1)}))  \ge$$
$$\sum_{i=1}^{\nexp} ELBO(x^{(i)}; Q^{(t)}, \theta^{(t)}) + \alpha \sum_{i=1}^{\nexp} LL(\tilde{x}^{(i)}, \tilde{z}^{(i)}; \theta^{(t)}) = \ell_\text{semi-sup}(\theta^{(t)})$$
\end{answer}
>>>>>>> dc304d27ca644bcbca0dc867837b32d7de83fed6
