\begin{answer}
Latent variables: $Q_i^{(t)}(z^{(i)})$  \\
From notes: $Q_i(z^{(i)}=j) = p(z|x;\theta)$
$$Q_i(z^{(i)}=j) = p(z|x;\theta) = \frac{p(x^{(i)}|z^{(i)};\theta) p(z^{(i)})}{\sum_{z^{(i)}} p(x^{(i)}|z^{(i)})p(z^{(i)})} = $$
$$\frac{\frac{1}{(2\pi)^{d/2}|\Sigma_j|^{1/2}}  exp(-\frac{(x^{(i)} - \mu_{z^{(i)}})^T \Sigma_{z^{(i)}}^{-1}(x^{(i)} - \mu_{z^{(i)}}) }{2})}
{\sum_{z^{(i)}}\frac{1}{(2\pi)^{d/2}|\Sigma_j|^{1/2}}  exp(-\frac{(x^{(i)} - \mu_{z^{(i)}})^T \Sigma_{z^{(i)}}^{-1}(x^{(i)} - \mu_{z^{(i)}}) }{2})} = $$
$$\frac{\frac{1}{|\Sigma_j|^{1/2}}  exp(-\frac{(x^{(i)} - \mu_{z^{(i)}})^T \Sigma_{z^{(i)}}^{-1}(x^{(i)} - \mu_{z^{(i)}}) }{2})}
{\sum_{z^{(i)}}\frac{1}{|\Sigma_j|^{1/2}}  exp(-\frac{(x^{(i)} - \mu_{z^{(i)}})^T \Sigma_{z^{(i)}}^{-1}(x^{(i)} - \mu_{z^{(i)}}) }{2})} $$
\end{answer}
