\begin{answer}
To re-estimate: $\phi, \mu, \Sigma$.
Firstly, let's write all this maximization problem:
$$\hat{\phi},\hat{\mu},\hat{\Sigma} = \arg\max_{\phi, \mu, \Sigma} \sum_{i=1}^{\nexp} ELBO(x^{(i)}, Q_i; \phi, \mu, \Sigma) = $$
$$ \arg\max_{\phi, \mu, \Sigma} \sum_{i=1}^{\nexp} \sum_{j=1}^{K} w_j^{(i)} \log \frac{p(x^{(i)}|z^{(i)}=j)p(z^{(i)}=j)}{w_j^{(i)}} +  \alpha \sum_{i=1}^{\tilde{\nexp}} \log(p(\tilde{x}^{(i)}, \tilde{z}^{(i)}; \phi, \mu, \Sigma)) = $$
$$\arg\max_{\phi, \mu, \Sigma} \sum_{i=1}^{\nexp} \sum_{j=1}^{K} w_j^{(i)} [\log p(x^{(i)}|z^{(i)}=j) + \log p(z^{(i)}=j)  - \log w_j^{(i)}] +  \alpha \sum_{i=1}^{\tilde{\nexp}} \log(p(\tilde{x}^{(i)} | \tilde{z}^{(i)}; \mu, \Sigma)) + $$
$$\alpha \sum_{i=1}^{\tilde{\nexp}} \log(p(\tilde{z}^{(i)}; \phi)) = $$
$$\arg\max_{\phi, \mu, \Sigma} \sum_{i=1}^{\nexp} \sum_{j=1}^{K} w_j^{(i)} [-\frac{1}{2}\log((2\pi)^{d} |\Sigma_j|) -  w_j^{(i)}\frac{(x^{(i)} - \mu_j)^T\Sigma_j^{-1}(x^{(i)} - \mu_j)}{2} + w_j^{(i)} \log \phi_j  -  w_j^{(i)}\log w_j^{(i)}] - $$
$$ \alpha \sum_{i=1}^{\tilde{\nexp}} \frac{1}{2}\log((2\pi)^{d} |\Sigma_{\tilde{z}^{(i)}}|) - \alpha \sum_{i=1}^{\tilde{\nexp}} \frac{(x^{(i)} - \mu_{\tilde{z}^{(i)}})^T\Sigma_{\tilde{z}^{(i)}}^{-1}(x^{(i)} - \mu_{\tilde{z}^{(i)}})}{2} + \alpha \sum_{i=1}^{\tilde{\nexp}} \log \phi_{\tilde{z}^{(i)}}$$

Let's find $\hat{\phi}$
$$\hat{\phi} =  \arg\max_{\phi} \sum_{i=1}^{\nexp} \sum_{j=1}^{K} w_j^{(i)} \log \phi_j +\alpha \sum_{i=1}^{\tilde{\nexp}} \sum_{j=1}^{\tilde{K}}\log \phi_{j} 1\{\tilde{z}^{(i)}=j\}$$
$$\nabla_{\phi_j}[\sum_{i=1}^{\nexp} \sum_{j=1}^{K} w_j^{(i)} \phi_j + \alpha \sum_{i=1}^{\tilde{\nexp}} \sum_{j=1}^{\tilde{K}} \phi_{j} 1\{\tilde{z}^{(i)}=j\} + \lambda ( \sum_{i=1}^{K} w_j^{(i)} -1)] = 0$$
$$\sum_{i=1}^{\nexp} w_j^{(i)} \frac{1}{\phi_j} +\alpha \sum_{i=1}^{\tilde{\nexp}} \frac{1}{\phi_{j}} 1\{\tilde{z}^{(i)}=j\} + \lambda = 0$$
$$\hat{\phi} = \frac{\sum_{i=1}^{\nexp} w_j^{(i)} +\alpha \sum_{i=1}^{\tilde{\nexp}} 1\{\tilde{z}^{(i)}=j\}}{-\lambda}$$
$$1 = \sum_{i=1}^{K} w_j^{(i)}=\sum_{i=1}^{K} \frac{\sum_{i=1}^{\nexp} w_j^{(i)} +\alpha \sum_{i=1}^{\tilde{\nexp}} 1\{\tilde{z}^{(i)}=j\}}{-\lambda}$$
$$\lambda = -[\sum_{i=1}^{\nexp} \sum_{i=1}^{K} w_j^{(i)} +\alpha \sum_{i=1}^{\tilde{\nexp}} \sum_{i=1}^{K} 1\{\tilde{z}^{(i)}=j\}] = -(n  + \alpha \tilde{n})$$
$$\hat{\phi} = \frac{\sum_{i=1}^{\nexp} w_j^{(i)} +\alpha \sum_{i=1}^{\tilde{\nexp}} 1\{\tilde{z}^{(i)}=j\}}{n  + \alpha \tilde{n}}$$

Let's find $\hat{\mu}$
$$\hat{\mu} =  \arg\max_{\mu} [- \sum_{i=1}^{\nexp} \sum_{j=1}^{K}  w_j^{(i)} \frac{(x^{(i)} - \mu_j)^T\Sigma_j^{-1}(x^{(i)} - \mu_j)}{2}  - \alpha \sum_{i=1}^{\tilde{\nexp}} \sum_{j=1}^{K} \frac{(\tilde{x}^{(i)} - \mu_{j})^T\Sigma_{j}^{-1}(\tilde{x}^{(i)} - \mu_{j})}{2} 1\{\tilde{z}^{(i)}=j\}] = $$
$$\nabla_{\mu_j}[\sum_{i=1}^{\nexp} \sum_{j=1}^{K} w_j^{(i)} (2\Sigma_j^{-1}) (x^{(i)} - \mu_j) +\alpha \sum_{i=1}^{\tilde{n}} \sum_{j=1}^{K}  1\{\tilde{z}^{(i)}=j\} (2\Sigma_j^{-1}) (\tilde{x}^{(i)} - \mu_j) ] = 0$$
$$\sum_{i=1}^{\nexp} w_j^{(i)} x^{(i)} - \sum_{i=1}^{\nexp}  w_j^{(i)} \mu_j +\alpha \sum_{i=1}^{\tilde{n}} \tilde{x}^{(i)} 1\{\tilde{z}^{(i)}=j\}-\alpha \mu_j \tilde{n} = 0$$
$$\mu_j = \frac{\sum_{i=1}^{\nexp}  w_j^{(i)} x^{(i)} + \alpha \sum_{i=1}^{\tilde{n}} \tilde{x}^{(i)}1\{\tilde{z}^{(i)}=j\}}{\sum_{i=1}^{\nexp} w_j^{(i)} + \alpha \tilde{n}}$$

Let's find $\hat{\Sigma}$
$$\hat{\Sigma} =  \arg\max_{\Sigma} [- \sum_{i=1}^{\nexp} \sum_{j=1}^{K}  w_j^{(i)} \frac{(x^{(i)} - \mu_j)^T\Sigma_j^{-1}(x^{(i)} - \mu_j)}{2}  - \alpha \sum_{i=1}^{\tilde{\nexp}} \sum_{j=1}^{K} \frac{(\tilde{x}^{(i)} - \mu_{j})^T\Sigma_{j}^{-1}(\tilde{x}^{(i)} - \mu_{j})}{2} 1\{\tilde{z}^{(i)}=j\}]$$ \\
$$ - \sum_{i=1}^{\nexp} \log(|\Sigma_{z^{(i)}}|)  - \sum_{i=1}^{\tilde{\nexp}} \log(|\Sigma_{\tilde{z}^{(i)}}|)]$$
$$-\sum_{i=1}^{\nexp} w_j^{(i)} \Sigma_j + \sum_{i=1}^{\nexp} \sum_{j=1}^{K}  w_j^{(i)} (x^{(i)} - \mu_j)(x^{(i)} - \mu_j)^T -  \alpha \sum_{i=1}^{\tilde{\nexp}} \Sigma_j 1\{\tilde{z}^{(i)}= j\} +  $$ \\
$$\alpha \sum_{i=1}^{\tilde{\nexp}} \sum_{j=1}^{K} (\tilde{x}^{(i)} - \mu_{j})(\tilde{x}^{(i)} - \mu_{j})^T 1\{\tilde{z}^{(i)}=j\}=0$$
$$\Sigma_j = \frac{ \sum_{i=1}^{\nexp} \sum_{j=1}^{K}  w_j^{(i)} (x^{(i)} - \mu_j)(x^{(i)} - \mu_j)^T + \alpha \sum_{i=1}^{\tilde{\nexp}} \sum_{j=1}^{K} (\tilde{x}^{(i)} - \mu_{j})(\tilde{x}^{(i)} - \mu_{j})^T 1\{\tilde{z}^{(i)}=j\}}{\sum_{i=1}^{\nexp} w_j^{(i)} + \alpha \sum_{i=1}^{\tilde{\nexp}} 1\{\tilde{z}^{(i)}= j\} }$$


\end{answer}
