\begin{answer}

\begin{equation*}
\int b(y)\exp(\eta^TT(y) - a(\eta)) dy = 1;
\int \frac{\partial}{\partial \eta}  b(y)\exp(\eta^TT(y) - a(\eta)) dy = 0 = 
\end{equation*}

\begin{equation*}
\int b(y)\exp(\eta^TT(y) - a(\eta))(y - \frac{\partial}{\partial\eta}a(\eta)) dy = 
\end{equation*}

\begin{equation*}
\int b(y)\exp(\eta^TT(y) - a(\eta))ydy - \frac{\partial}{\partial\eta}a(\eta) \int b(y)\exp(\eta^TT(y) - a(\eta))dy.
\end{equation*}

\begin{equation*}
\mathbb{E}[Y; \eta]  - \frac{\partial}{\partial\eta}a(\eta) * 1 = 0.
\end{equation*}



\end{answer}
