\begin{answer}

\begin{equation*}
\ell(\theta) = - \log(\prod_{i=1}^\nexp b(y^{(i)} e^{\eta y^{(i)} - a(\eta)})) = - \log(\prod_{i=1}^\nexp b(y^{(i)})) - \log(\prod_{i=1}^\nexp e^{\eta y^{(i)} - a(\eta)}) 
\end{equation*}

\begin{equation*}
\nabla_\theta \ell(\theta) = - \sum_{i=1}^\nexp x^{(i)} (y^{(i)} - \frac{\partial}{\partial\eta}a(\eta)) x^{(i)} = - \sum_{i=1}^\nexp x^{(i)} (y^{(i)} - \frac{\partial}{\partial\eta}a(\eta)))
\end{equation*}

\begin{equation*}
\nabla_\theta \frac{\partial}{\partial\eta}\ell(\eta_{j})) = - \sum_{i=1}^\nexp x_{j}^{(i)} (-Var[y|x^{(i)}; \theta]) * x^{(i)} = \sum_{i=1}^\nexp x_{j}^{(i)} (Var[y|x^{(i)}; \theta]) * x^{(i)}
\end{equation*}


\begin{equation*}
z^THz = \sum_{i=1}^\nexp Var[y|x^{(i)}; \theta] * (x^{(i)}*z)^{2} \ge 0
\end{equation*}



\end{answer}
