\begin{answer}

\begin{equation*}
\log p(y^{(i)} | x^{(i)}; \theta) = \log(\frac{e^{-\lambda} \lambda^{y^{(i)}}}{y^{(i)}!}) = 
y^{(i)}\log(y^{(i)}!)e^{\theta^Tx^{(i)}}\theta^Tx^{(i)}
\end{equation*}

\begin{equation*}
\nabla_\theta \sum_{i=1}^\nexp(\log p(y^{(i)} | x^{(i)}; \theta)) = \sum_{i=1}^\nexp y^{(i)}\log(y^{(i)}!) e^{\theta^Tx^{(i)}} * x^{(i)} (1 + \theta^Tx^{(i)})
\end{equation*}

\begin{equation*}
\theta = \theta + \alpha \nabla_\theta \sum_{i=1}^\nexp(\log p(y^{(i)} | x^{(i)}; \theta)) 
\end{equation*}


\end{answer}
